RelationalAlgebra/Util.lean
@@ -5,11 +5,13 @@ open RM
 section empty
 
 @[simp]
-def emptyInst {schema : RelationSchema} : RelationInstance := ⟨
+abbrev RelationInstance.empty (schema : RelationSchema) : RelationInstance := ⟨
   schema,
   ∅,
   by simp only [Set.mem_empty_iff_false, IsEmpty.forall_iff, implies_true]
 ⟩
+
+prefix:100 "∅r " => RelationInstance.empty
 
 end empty
 
